a re-implementation of exprUnify that avoids Fix.

src/ExprUnify.v
@@ -674,316 +674,155 @@ Module SynUnifier (E : OrderedType.OrderedType with Definition t := uvar with De
 
     End fold_in.
 
-    Definition exprUnify_recursor bound_l 
-      (recur : forall a_b, R_pair GenRec.R_nat (@R_expr types) a_b bound_l -> expr types -> Subst -> option Subst)
-      (r : expr types) (sub : Subst) : option Subst.
-    refine (
-      match bound_l as bound_l
-        return (forall a_b, R_pair GenRec.R_nat (@R_expr types) a_b bound_l -> expr types -> Subst -> option Subst)
-        -> option Subst
-        with
-        | (bound,l) =>
-          match l as l , r as r 
-            return (forall a_b, R_pair GenRec.R_nat (@R_expr types) a_b (bound, l) -> expr types -> Subst -> option Subst)
-            -> option Subst
-            with
-            | Const t v , Const t' v' => fun _ =>
-              match equiv_dec t t' with
-                | left pf => match pf in _ = k return tvarD _ k -> _ with
-                               | refl_equal => fun v' =>
-                                 if get_Eq types t v v'
-                                   then Some sub
-                                   else None
-                             end v'
-                | right _ => None
+    Section unify.
+      Variable exprUnify : expr types -> expr types -> Subst -> option Subst.
+
+      Fixpoint unify (l r : expr types) (sub : Subst) : option Subst :=
+        match l , r with
+          | Const t v , Const t' v' => 
+            match equiv_dec t t' with
+              | left pf => match pf in _ = k return tvarD _ k -> _ with
+                             | refl_equal => fun v' =>
+                               if get_Eq types t v v'
+                                 then Some sub
+                                 else None
+                           end v'
+              | right _ => None
+            end
+          | Var v , Var v' => 
+            if Peano_dec.eq_nat_dec v v' 
+              then Some sub
+              else None
+          | Func f1 args1 , Func f2 args2 =>
+            if EqNat.beq_nat f1 f2 then
+              (fix unifyArgs (args1 args2 : list (expr types)) (s : Subst) 
+                : option Subst :=
+                match args1 , args2 with
+                  | nil , nil => Some s
+                  | nil , _ :: _ => None
+                  | _ :: _ , nil => None
+                  | arg1 :: args1 , arg2 :: args2 =>
+                    match unify arg1 arg2 s with
+                      | None => None
+                      | Some s => unifyArgs args1 args2 s
+                    end
+                end) args1 args2 sub
+              else None
+          | Equal t1 e1 f1 , Equal t2 e2 f2 =>
+            if equiv_dec t1 t2 then
+              match unify e1 e2 sub with
+                | None => None
+                | Some sub => unify f1 f2 sub
               end
-            | Var v , Var v' => fun _ => 
+              else
+                None
+          | Not e1 , Not e2 =>
+            unify e1 e2 sub
+          | UVar l , UVar r => 
+            if EqNat.beq_nat l r then Some sub
+              else 
+                match Subst_lookup l sub with
+                  | None => Subst_set l (UVar r) sub
+                  | Some l' =>
+                    match Subst_lookup r sub with
+                      | None => Subst_set r l' sub
+                      | Some r' =>
+                        exprUnify l' r' sub
+                    end
+                end
+          | UVar u , r =>
+            match Subst_lookup u sub with
+              | None =>
+                Subst_set u r sub
+              | Some l' =>
+                exprUnify l' r sub
+            end
+          | l , UVar u =>
+            match Subst_lookup u sub with
+              | None => 
+                Subst_set u l sub
+              | Some r' =>
+                exprUnify l r' sub
+            end
+          | _ , _ => None
+        end.
+    End unify.
+      
+
+    Fixpoint exprUnify (bound : nat) : expr types -> expr types -> Subst -> option Subst :=
+      match bound with 
+        | 0 => fun _ _ _ => None
+        | S bound =>
+          fix unify (l r : expr types) (sub : Subst) : option Subst :=
+            match l , r with
+              | Const t v , Const t' v' => 
+                match equiv_dec t t' with
+                  | left pf => match pf in _ = k return tvarD _ k -> _ with
+                                 | refl_equal => fun v' =>
+                                   if get_Eq types t v v'
+                                     then Some sub
+                                     else None
+                               end v'
+                  | right _ => None
+                end
+            | Var v , Var v' => 
               if Peano_dec.eq_nat_dec v v' 
                 then Some sub
                 else None
-            | Func f1 args1 , Func f2 args2 => fun recur =>
+            | Func f1 args1 , Func f2 args2 =>
               if EqNat.beq_nat f1 f2 then
-                @dep_in args1 (fun l r s pf => recur (bound, l) _ r s) args1 args2 sub (fun _ pf => pf)
+                (fix unifyArgs (args1 args2 : list (expr types)) (s : Subst) 
+                  : option Subst :=
+                  match args1 , args2 with
+                    | nil , nil => Some s
+                    | nil , _ :: _ => None
+                    | _ :: _ , nil => None
+                    | arg1 :: args1 , arg2 :: args2 =>
+                      match unify arg1 arg2 s with
+                        | None => None
+                        | Some s => unifyArgs args1 args2 s
+                      end
+                  end) args1 args2 sub
               else None
-            | Equal t1 e1 f1 , Equal t2 e2 f2 => fun recur =>
+            | Equal t1 e1 f1 , Equal t2 e2 f2 =>
               if equiv_dec t1 t2 then
-                match recur (bound, e1) _ e2 sub with
+                match unify e1 e2 sub with
                   | None => None
-                  | Some sub => recur (bound, f1) _ f2 sub
+                  | Some sub => unify f1 f2 sub
                 end
-                else
-                  None
-            | Not e1 , Not e2 => fun recur =>
-              recur (bound,e1) _ e2 sub
+              else
+                None
+            | Not e1 , Not e2 =>
+              unify e1 e2 sub
             | UVar l , UVar r => 
-              if EqNat.beq_nat l r then fun _ => Some sub
+              if EqNat.beq_nat l r then Some sub
               else 
                 match Subst_lookup l sub with
-                  | None => fun _ => Subst_set l (UVar r) sub
+                  | None => Subst_set l (UVar r) sub
                   | Some l' =>
                     match Subst_lookup r sub with
-                      | None => fun _ => Subst_set r l' sub
+                      | None => Subst_set r l' sub
                       | Some r' =>
-                        match bound as bound return 
-                          (forall a_b, R_pair GenRec.R_nat (@R_expr types) a_b (bound,UVar l) -> expr types -> Subst -> option Subst)
-                          -> option Subst with
-                          | 0 => fun _ => None
-                          | S bound => fun recur => recur (bound, l') _ r' sub
-                        end
+                        exprUnify bound l' r' sub
                     end
                 end
-            | UVar u , _ =>
+            | UVar u , r =>
               match Subst_lookup u sub with
-                | None => fun recur =>
+                | None =>
                   Subst_set u r sub
                 | Some l' =>
-                  match bound as bound return 
-                    (forall a_b, R_pair GenRec.R_nat (@R_expr types) a_b (bound,UVar u) -> expr types -> Subst -> option Subst)
-                    -> option Subst with
-                    | 0 => fun _ => None
-                    | S bound => fun recur => recur (bound, l') _ r sub
-                  end
+                  exprUnify bound l' r sub
               end
             | l , UVar u =>
               match Subst_lookup u sub with
-                | None => fun recur =>
+                | None => 
                   Subst_set u l sub
                 | Some r' =>
-                  match bound as bound return 
-                    (forall a_b, R_pair GenRec.R_nat (@R_expr types) a_b (bound,l) -> expr types -> Subst -> option Subst)
-                    -> option Subst with
-                    | 0 => fun _ => None
-                    | S bound => fun recur => recur (bound, l) _ r' sub
-                  end
+                  exprUnify bound l r' sub
               end
-            | _ , _ => fun _ => None
-          end 
-      end recur
-    ); try solve [ apply GenRec.L ; constructor | apply GenRec.R ; constructor; assumption ].
-    Defined.
-
-    (** index by a bound, since the termination argument is not trivial
-     ** it is guaranteed to not make more recursions than the number of
-     ** uvars.
-     **)
-    Definition exprUnify (bound : nat) (l : expr types) : expr types -> Subst -> option Subst :=
-      (@Fix _ _ (guard 4 (GenRec.wf_R_pair GenRec.wf_R_nat (@wf_R_expr types)))
-        (fun _ => expr types -> Subst -> option Subst) exprUnify_recursor) (bound,l).
-
-    (** Proofs **)
-    Section equiv.
-      Variable A : Type.
-      Variable R : A -> A -> Prop.
-      Hypothesis Rwf : well_founded R.
-      Variable P : A -> Type.
-      
-      Variable equ : forall x, P x -> P x -> Prop.
-      Hypothesis equ_Equiv : forall x, RelationClasses.Equivalence (@equ x).
-      
-      Variable F : forall x : A, (forall y : A, R y x -> P y) -> P x.
-
-      Lemma Fix_F_equ : forall (x : A) (r : Acc R x),
-        equ (@F x (fun (y : A) (p : R y x) => Fix_F P F (Acc_inv r p)))
-        (Fix_F P F r).
-      Proof.
-        eapply Acc_inv_dep; intros.
-        simpl in *. reflexivity.
-      Qed.
-
-      Lemma Fix_F_inv_equ : 
-        (forall (x : A) (f g : forall y : A, R y x -> P y),
-          (forall (y : A) (p : R y x), equ (@f y p) (g y p)) -> equ (@F x f) (@F x g)) ->
-        forall (x : A) (r s : Acc R x), equ (Fix_F P F r) (Fix_F P F s).
-      Proof.
-        intro. intro. induction (Rwf x). intros.
-        erewrite <- Fix_F_equ. symmetry. erewrite <- Fix_F_equ. symmetry.
-        eapply H. intros. eauto.
-      Qed.
-
-    End equiv.
-
-    Lemma Equiv_equiv : Equivalence
-      (fun f g : expr types -> Subst -> option Subst =>
-        forall (a : expr types) (b : Subst), f a b = g a b).
-    Proof.
-      constructor; eauto.
-      red. intros. rewrite H; eauto.
-    Qed.
-
-    Lemma exprUnify_recursor_inv : forall (bound : nat)
-      e1 e2 (sub : Subst) (A B : Acc _ (bound,e1))
-      (w : well_founded (R_pair R_nat (R_expr (ts:=types)))),
-      Fix_F (fun _ : nat * expr types => expr types -> Subst -> option Subst)
-      exprUnify_recursor A e2 sub =
-      Fix_F (fun _ : nat * expr types => expr types -> Subst -> option Subst)
-      exprUnify_recursor B e2 sub.
-    Proof.
-      intros.
-      eapply (@Fix_F_inv_equ (nat * expr types) (R_pair R_nat (R_expr (ts:=types)))
-        w
-        (fun _ : nat * expr types => expr types -> Subst -> option Subst)
-        (fun x f g => forall a b, f a b = g a b)
-        (fun _ => Equiv_equiv)
-        exprUnify_recursor).
-      clear. intros.
-      unfold exprUnify_recursor. destruct x. destruct e; destruct a; auto;
-      repeat match goal with 
-               | _ => reflexivity
-               | [ H : _ |- _ ] => rewrite H
-               | [ |- context [ match ?X with 
-                                  | _ => _
-                                end ] ] => destruct X
-             end.
-      generalize (fun (l1 : expr types) (pf : In l1 l) => pf).
-      assert (
-        forall l' l0 b, forall i : forall l1 : expr types, In l1 l' -> In l1 l,
-          dep_in l
-          (fun (l1 r0 : expr types) (s : Subst) (pf : In l1 l) =>
-            f (n, l1)
-            (R R_nat (R_expr (ts:=types)) n l1 (Func f0 l) (R_Func f0 l l1 pf))
-            r0 s) l' l0 b i =
-          dep_in l
-          (fun (l1 r0 : expr types) (s : Subst) (pf : In l1 l) =>
-            g (n, l1)
-            (R R_nat (R_expr (ts:=types)) n l1 (Func f0 l) (R_Func f0 l l1 pf))
-            r0 s) l' l0 b i).
-      induction l'; simpl in *; intros; auto.
-      destruct l1; auto. 
-      rewrite H. destruct (g (n, a)); auto.
-      eapply H0.
-    Qed.
-
-    Theorem exprUnify_unroll : forall bound l r sub,
-      exprUnify bound l r sub = 
-      match l , r with
-        | Const t v , Const t' v' =>
-          match equiv_dec t t' with
-            | left pf => match pf in _ = k return tvarD _ k -> _ with
-                           | refl_equal => fun v' =>
-                             if get_Eq types t v v'
-                               then Some sub
-                               else None
-                         end v'
-            | right _ => None
-          end
-        | Var v , Var v' => 
-          if Peano_dec.eq_nat_dec v v' 
-            then Some sub
-            else None
-        | Func f1 args1 , Func f2 args2 =>
-          if EqNat.beq_nat f1 f2 then
-            Folds.fold_left_2_opt (@exprUnify bound) args1 args2 sub
-          else None
-        | Equal t1 e1 f1 , Equal t2 e2 f2 =>
-          if equiv_dec t1 t2 then
-            match exprUnify bound e1 e2 sub with
-              | None => None
-              | Some sub => exprUnify bound f1 f2 sub
+            | _ , _ => None
             end
-            else
-              None
-        | Not e1, Not e2 =>
-          exprUnify bound e1 e2 sub
-        | UVar l , UVar r => 
-          if EqNat.beq_nat l r then Some sub
-            else 
-              match Subst_lookup l sub with
-                | None => Subst_set l (UVar r) sub
-                | Some l' =>
-                  match Subst_lookup r sub with
-                    | None => Subst_set r l' sub
-                    | Some r' =>
-                      match bound with
-                        | 0 => None
-                        | S bound => exprUnify bound l' r' sub
-                      end
-                  end
-              end
-        | UVar u , _ =>
-          match Subst_lookup u sub with
-            | None => Subst_set u r sub
-            | Some l' =>
-              match bound with
-                | 0 => None
-                | S bound => exprUnify bound l' r sub
-              end
-          end
-        | l , UVar u =>
-          match Subst_lookup u sub with
-            | None => Subst_set u l sub
-            | Some r' =>
-              match bound with
-                | 0 => None
-                | S bound => exprUnify bound l r' sub
-              end
-          end
-        | _ , _ => None
       end.
-    Proof.
-      intros. unfold exprUnify at 1.
-      match goal with
-        | [ |- context [ guard ?X ?Y ] ] =>
-          generalize (guard X Y)
-      end.
-      intros. unfold Fix.
-      rewrite <- (@Fix_F_equ (nat * expr types) (R_pair R_nat (R_expr (ts:=types)))
-        (fun _ : nat * expr types => expr types -> Subst -> option Subst)
-        (fun x f g => forall a b, f a b = g a b)
-        (fun _ => Equiv_equiv)
-        exprUnify_recursor
-        (bound,l)
-        (w (bound,l))
-        r sub).
-      destruct l; destruct r; simpl; intros; auto;
-        try solve [
-          repeat match goal with
-                   | [ |- context [ match ?X with 
-                                      | _ => _ 
-                                    end ] ] => destruct X
-                 end; try solve [ auto | 
-                   unfold exprUnify, Fix ;
-                     eapply exprUnify_recursor_inv; eauto ] ].
-      Focus 2.
-      destruct (equiv_dec t t0); auto.
-      unfold exprUnify, Fix.
-      erewrite exprUnify_recursor_inv; eauto.
-      instantiate (1 := (guard 4 (wf_R_pair wf_R_nat (wf_R_expr (ts:=types))) (bound, l1))).
-      match goal with 
-        | [ |- match ?X with 
-                 | _ => _ 
-               end = _ ] => destruct X
-      end; auto.
-      erewrite exprUnify_recursor_inv; eauto.
-
-      match goal with
-        | [ |- match ?X with
-                 | _ => _
-               end = _ ] => destruct X; auto
-      end.
-      generalize (fun (l1 : expr types) (pf : In l1 l) => pf).
-      assert (forall l' l0 sub,
-        forall i : (forall l1 : expr types, In l1 l' -> In l1 l),
-          dep_in l
-          (fun (l1 r0 : expr types) (s : Subst) (pf : In l1 l) =>
-            @Fix_F _ _ (fun _ : nat * expr types => expr types -> Subst -> option Subst)
-            exprUnify_recursor (bound, l1) (@Acc_inv (nat * expr types)
-              (@R_pair nat (expr types) R_nat (@R_expr types))
-              (bound, @Func types f l) (w (bound, @Func types f l)) 
-              (bound, l1)
-              (@R nat (expr types) R_nat (@R_expr types) bound l1
-                (@Func types f l) (@R_Func types f l l1 pf))) r0 s) l' l0 sub i =
-          Folds.fold_left_2_opt (exprUnify bound) l' l0 sub).
-      induction l'; simpl; intros; destruct l1; auto.
-      erewrite exprUnify_recursor_inv; eauto.
-      instantiate (1 := (guard 4 (wf_R_pair wf_R_nat (wf_R_expr (ts:=types))) (bound, a))).
-      unfold exprUnify, Fix.
-      match goal with
-        | [ |- match ?X with
-                 | _ => _
-               end = _ ] => destruct X; auto
-      end.
-      eapply H.
-    Qed.
 
     Lemma Subst_set_Subst_lookup : forall k v sub sub',
       Subst_set k v sub = Some sub' ->
@@ -1013,7 +852,6 @@ Module SynUnifier (E : OrderedType.OrderedType with Definition t := uvar with De
       { f_equal. induction H; simpl; intros; think; auto. }
     Qed.
 
-
     Lemma Subst_set_Extends : forall k v sub sub',
       Subst_set k v sub = Some sub' ->
       Subst_lookup k sub = None ->
@@ -1039,53 +877,6 @@ Module SynUnifier (E : OrderedType.OrderedType with Definition t := uvar with De
           eapply adf; eauto.
     Qed.
 
-    Lemma fold_left_2_opt_exprUnify_Extends' : forall b l l0 sub sub',
-      Folds.fold_left_2_opt (exprUnify b) l l0 sub = Some sub' ->
-      Forall
-      (fun l : expr types =>
-        forall (r : expr types) (sub sub' : Subst),
-          exprUnify b l r sub = Some sub' -> Subst_Extends sub' sub) l ->
-      Subst_Extends sub' sub.
-    Proof.
-      intros.
-      generalize dependent l0. generalize dependent sub.
-      induction H0; destruct l0; simpl in *; try congruence; intros.
-        inversion H; eapply Refl_Subst_Extends.
-
-      revert H1; case_eq (exprUnify b x e sub); try congruence; intros.
-      eapply Trans_Subst_Extends; eauto. 
-    Qed.
-
-    Theorem exprUnify_Extends : forall n l r sub sub',
-      exprUnify n l r sub = Some sub' ->
-      Subst_Extends sub' sub.
-    Proof.
-      induction n; induction l; intros; rewrite exprUnify_unroll in *; destruct r; simpl in *;
-        try solve [ 
-          repeat (congruence || eauto ||
-              solve [ eapply Subst_set_Extends; eauto |
-                      eapply Trans_Subst_Extends; eauto |
-                      apply Refl_Subst_Extends |
-                  eapply fold_left_2_opt_exprUnify_Extends'; eauto ] ||
-              match goal with
-                | [ H : Equivalence.equiv _ _ |- _ ] => 
-                  unfold Equivalence.equiv in H; subst
-                | [ H : Some _ = Some _ |- _ ] => inversion H; clear H; subst
-                | [ H : match exprUnify ?A ?B ?C ?D with _ => _ end = _ |- _ ] => 
-                  revert H; case_eq (exprUnify A B C D); intros
-                | [ H : match ?X with _ => _ end = _ |- _ ] => revert H; case_eq X; intros
-              end) ].
-    Qed.
-
-    Lemma fold_left_2_opt_exprUnify_Extends : forall b l l0 sub sub',
-      Folds.fold_left_2_opt (exprUnify b) l l0 sub = Some sub' ->
-      Subst_Extends sub' sub.
-    Proof.
-      induction l; destruct l0; simpl in *; try congruence; intros.
-        inversion H; subst; apply Refl_Subst_Extends.
-      revert H; case_eq (exprUnify b a e sub); try congruence; intros.
-      eapply Trans_Subst_Extends; eauto using exprUnify_Extends.
-    Qed.
 
     Lemma Subst_lookup_Extends : forall sub sub' k v,
       Subst_lookup k sub = Some v ->
@@ -1106,22 +897,6 @@ Module SynUnifier (E : OrderedType.OrderedType with Definition t := uvar with De
       intros.
       cut (exprInstantiate sub' (exprInstantiate sub l) = exprInstantiate sub' (exprInstantiate sub r)); intros.
       repeat (rewrite exprInstantiate_Extends in H1; eauto). rewrite H; reflexivity.
-    Qed.
-
-    Lemma fold_left_2_opt_map_sound' : forall (n : nat) (l l0 : list (expr types)) (sub sub' : Subst),
-      Folds.fold_left_2_opt (exprUnify n) l l0 sub = Some sub' ->
-      Forall
-      (fun l1 : expr types =>
-        forall (r : expr types) (sub0 sub'0 : Subst),
-          exprUnify n l1 r sub0 = Some sub'0 ->
-          exprInstantiate sub'0 l1 = exprInstantiate sub'0 r) l ->
-      map (exprInstantiate sub') l = map (exprInstantiate sub') l0.
-    Proof.
-      intros.
-      generalize dependent l0. revert sub; revert sub'. 
-      induction H0; simpl in *; intros; destruct l0; simpl in *; try congruence; auto.
-      revert H1. case_eq (exprUnify n x e sub); intros; try congruence.
-      f_equal; eauto using exprInstantiate_extends, exprUnify_Extends, fold_left_2_opt_exprUnify_Extends.
     Qed.
 
     Lemma Subst_set_exprInstantiate : forall x e sub sub',
@@ -1213,114 +988,6 @@ Module SynUnifier (E : OrderedType.OrderedType with Definition t := uvar with De
       destruct l0; auto; simpl in *.
       rewrite <- IHForall. rewrite <- H. reflexivity.
     Qed. 
-
-    Opaque Subst_lookup Subst_set exprInstantiate.
-
-    Theorem exprUnify_sound : forall n l r sub sub',
-      exprUnify n l r sub = Some sub' ->
-      exprInstantiate sub' l = exprInstantiate sub' r.
-    Proof.
-      induction n; induction l; intros; rewrite exprUnify_unroll in *; destruct r; simpl in *;
-        try solve [ 
-          repeat (congruence || 
-                  solve [ eauto |
-                          eapply exprInstantiate_extends; eauto using exprUnify_Extends |
-                          eapply fold_left_2_opt_map_sound'; eauto ] ||
-              match goal with
-                | [ H : Equivalence.equiv _ _ |- _ ] => 
-                  unfold Equivalence.equiv in H; subst
-                | [ |- _ ] => erewrite Subst_set_exprInstantiate by eauto
-                | [ H : _ |- _ ] => erewrite H by eauto
-                | [ |- _ ] => erewrite Subst_set_Subst_lookup by eauto
-                | [ H : forall (l r : expr types) (sub sub' : Subst), exprUnify _ l r sub = Some sub' -> _ , H' : _ |- _ ] =>
-                  specialize (@H _ _ _ _ H')
-                | [ H : Subst_lookup _ _ = _ |- _ ] =>
-                  eapply Subst_lookup_Extends in H; [ | solve [ eauto using exprUnify_Extends ] ]
-                | [ H : match exprUnify ?A ?B ?C ?D with _ => _ end = _ |- _ ] => 
-                  revert H; case_eq (exprUnify A B C D); intros
-                | [ H : match Subst_lookup ?X ?Y with _ => _ end = _ |- _ ] =>
-                  revert H; case_eq (Subst_lookup X Y); intros
-                | [ H : match ?X with _ => _ end = _ |- _ ] => 
-                  revert H; Reflection.consider X; intros
-                | [ |- Equal _ _ _ = Equal _ _ _ ] => f_equal
-                | [ |- Func _ _ = Func _ _ ] => f_equal
-                | [ |- _ ] => 
-                  rewrite exprInstantiate_Func || rewrite exprInstantiate_Equal ||
-                  rewrite exprInstantiate_Not || rewrite exprInstantiate_UVar ||
-                  rewrite exprInstantiate_Var || rewrite exprInstantiate_Const
-              end) ].
-      { repeat (congruence || 
-                  solve [ eauto |
-                          eapply exprInstantiate_extends; eauto using exprUnify_Extends |
-                          eapply fold_left_2_opt_map_sound'; eauto ] ||
-              match goal with
-                | [ H : Equivalence.equiv _ _ |- _ ] => 
-                  unfold Equivalence.equiv in H; subst
-                | [ |- _ ] => erewrite Subst_set_exprInstantiate by eauto
-                | [ H : _ |- _ ] => erewrite H by eauto
-                | [ |- _ ] => erewrite Subst_set_Subst_lookup by eauto
-                | [ H : forall (l r : expr types) (sub sub' : Subst), exprUnify _ l r sub = Some sub' -> _ , H' : _ |- _ ] =>
-                  specialize (@H _ _ _ _ H')
-                | [ H : Subst_lookup _ _ = _ |- _ ] =>
-                  eapply Subst_lookup_Extends in H; [ | solve [ eauto using exprUnify_Extends ] ]
-                | [ H : match exprUnify ?A ?B ?C ?D with _ => _ end = _ |- _ ] => 
-                  revert H; case_eq (exprUnify A B C D); intros
-                | [ H : match Subst_lookup ?X ?Y with _ => _ end = _ |- _ ] =>
-                  revert H; case_eq (Subst_lookup X Y); intros
-                | [ H : match ?X with _ => _ end = _ |- _ ] => 
-                  revert H; Reflection.consider X; intros
-                | [ |- Equal _ _ _ = Equal _ _ _ ] => f_equal
-                | [ |- Func _ _ = Func _ _ ] => f_equal
-                | [ |- _ ] => 
-                  rewrite exprInstantiate_Func || rewrite exprInstantiate_Equal ||
-                  rewrite exprInstantiate_Not || rewrite exprInstantiate_UVar ||
-                  rewrite exprInstantiate_Var || rewrite exprInstantiate_Const
-              end).
-        eapply Subst_set_Extends in H2; try eassumption.
-        erewrite Subst_lookup_Extends; try eassumption.
-        reflexivity. }
-      { repeat (congruence || 
-                  solve [ eauto |
-                          eapply exprInstantiate_extends; eauto using exprUnify_Extends |
-                          eapply fold_left_2_opt_map_sound'; eauto ] ||
-              match goal with
-                | [ H : Equivalence.equiv _ _ |- _ ] => 
-                  unfold Equivalence.equiv in H; subst
-                | [ |- _ ] => erewrite Subst_set_exprInstantiate by eauto
-                | [ H : _ |- _ ] => erewrite H by eauto
-                | [ |- _ ] => erewrite Subst_set_Subst_lookup by eauto
-                | [ H : forall (l r : expr types) (sub sub' : Subst), exprUnify _ l r sub = Some sub' -> _ , H' : _ |- _ ] =>
-                  specialize (@H _ _ _ _ H')
-                | [ H : Subst_lookup _ _ = _ |- _ ] =>
-                  eapply Subst_lookup_Extends in H; [ | solve [ eauto using exprUnify_Extends ] ]
-                | [ H : match exprUnify ?A ?B ?C ?D with _ => _ end = _ |- _ ] => 
-                  revert H; case_eq (exprUnify A B C D); intros
-                | [ H : match Subst_lookup ?X ?Y with _ => _ end = _ |- _ ] =>
-                  revert H; case_eq (Subst_lookup X Y); intros
-                | [ H : match ?X with _ => _ end = _ |- _ ] => 
-                  revert H; Reflection.consider X; intros
-                | [ |- Equal _ _ _ = Equal _ _ _ ] => f_equal
-                | [ |- Func _ _ = Func _ _ ] => f_equal
-                | [ |- _ ] => 
-                  rewrite exprInstantiate_Func || rewrite exprInstantiate_Equal ||
-                  rewrite exprInstantiate_Not || rewrite exprInstantiate_UVar ||
-                  rewrite exprInstantiate_Var || rewrite exprInstantiate_Const
-              end).
-        eapply Subst_set_Extends in H2; try eassumption.
-        erewrite Subst_lookup_Extends; try eassumption.
-        reflexivity. }
-    Qed.
-
-    Theorem exprUnify_sound' : forall n l r sub sub',
-      exprUnify n l r sub = Some sub' ->
-      forall funcs U G t,
-      exprD funcs U G (exprInstantiate sub' l) t = 
-      exprD funcs U G (exprInstantiate sub' r) t.
-    Proof.
-      intros. apply exprUnify_sound in H. rewrite H. reflexivity.
-    Qed.
-
-    Transparent Subst_set.
           
     Lemma Subst_set_WellTyped : forall funcs U G u E t sub sub',
       Subst_set u E sub = Some sub' ->
@@ -1379,69 +1046,212 @@ Module SynUnifier (E : OrderedType.OrderedType with Definition t := uvar with De
       apply FACTS.find_mapsto_iff in H. eapply H0 in H. destruct H. rewrite H1 in *. intuition.
       inversion H2; auto.
     Qed.
-    Opaque Subst_lookup.
 
-(*    SearchAbout is_well_typed.
+    Opaque Subst_lookup Subst_set exprInstantiate.
 
-    Lemma is_well_typed_const : forall funcs U G t (v : tvarD types t),
-      is_well_typed funcs U G (Const v) t = true.
+    Theorem unify_uvar : forall (u : uvar) (sub sub' : Subst)
+      (o : expr types -> expr types -> Subst -> option Subst),
+      (forall (l r : expr types) (sub0 sub'0 : Subst),
+        o l r sub0 = Some sub'0 ->
+        exprInstantiate sub'0 l = exprInstantiate sub'0 r /\
+        Subst_Extends sub'0 sub0 /\
+        (forall (funcs : tfunctions) (U G : tenv) (t : tvar),
+          is_well_typed funcs U G l t = true ->
+          is_well_typed funcs U G r t = true ->
+          Subst_WellTyped funcs U G sub0 -> Subst_WellTyped funcs U G sub'0)) ->
+      forall e : expr types,
+        match Subst_lookup u sub with
+          | Some r' => o e r' sub
+          | None => Subst_set u e sub
+        end = Some sub' ->
+        exprInstantiate sub' e = exprInstantiate sub' (UVar u) /\
+        Subst_Extends sub' sub /\
+        (forall (funcs : tfunctions) (U G : tenv) (t1 : tvar),
+          is_well_typed funcs U G e t1 = true ->
+          is_well_typed (types := types) funcs U G (UVar u) t1 = true ->
+          Subst_WellTyped funcs U G sub -> Subst_WellTyped funcs U G sub').
     Proof.
-      simpl. intros. consider (tvar_seqb t t); auto.
+      intros. consider (Subst_lookup u sub); intros.
+      { specialize (H _ _ _ _ H1). rewrite exprInstantiate_UVar.
+        intuition.
+        { erewrite Subst_lookup_Extends by eassumption. auto. }
+        { eapply H4; try eassumption.
+          eapply Subst_lookup_WellTyped; try eassumption. simpl in H5.
+          destruct (nth_error U u); try congruence.
+          consider (tvar_seqb t1 t); congruence. } }
+      { clear H; intuition. 
+        { erewrite Subst_set_exprInstantiate by eassumption; auto. }
+        { eapply Subst_set_Extends; eauto. }
+        { eapply Subst_set_WellTyped; try eassumption. simpl in H2.
+          destruct (nth_error U u); try congruence.
+          consider (tvar_seqb t1 t); congruence. } }
     Qed.
-    Lemma is_well_typed_var : forall funcs U G t v,
-      nth_error G v = Some t ->
-      is_well_typed funcs U G (@Var types v) t = true.
-    Proof.
-      simpl. intros; rewrite H. consider (tvar_seqb t t); auto. 
-    Qed.
-    Lemma is_well_typed_uvar : forall funcs U G t v,
-      nth_error U v = Some t ->
-      is_well_typed funcs U G (@UVar types v) t = true.
-    Proof.
-      simpl. intros; rewrite H. consider (tvar_seqb t t); auto. 
-    Qed.
-*)
 
-    Hint Extern 1 (is_well_typed _ _ _ _ _ = _) =>
-      simpl;
-        repeat match goal with 
-                 | [ H : _ = _ |- _ ] => rewrite H
-                 | [ |- _ ] => rewrite EquivDec_refl_left
-                 | [ |- _ ] => rewrite tvar_seqb_refl
-               end; reflexivity : exprs.
-(*
-    Hint Resolve is_well_typed_const is_well_typed_var is_well_typed_uvar : exprs. 
-        Hint Extern 1 (is_well_typed _ _ _ _ _ = true) => simpl; think : exprs.
-*)
-    
-    Lemma exprUnify_WellTyped_Forall : forall n (l : list (expr types)),
-      Forall
-      (fun l0 : expr types =>
-        forall (r : expr types) (sub sub' : Subst),
-          exprUnify n l0 r sub = Some sub' ->
-          forall (funcs : tfunctions) (U G : tenv) (t : tvar),
-            is_well_typed funcs U G l0 t = true ->
+    Lemma exprUnify_all : forall n l r sub sub',
+      exprUnify n l r sub = Some sub' ->
+         (exprInstantiate sub' l = exprInstantiate sub' r)
+      /\ (Subst_Extends sub' sub)
+      /\ (forall funcs U G t,
+            is_well_typed funcs U G l t = true ->
             is_well_typed funcs U G r t = true ->
-            Subst_WellTyped funcs U G sub -> Subst_WellTyped funcs U G sub') l ->
-      forall (funcs : tfunctions) (U G : tenv) (sub' : Subst) 
-        (l0 : list tvar) (sub : Subst),
-        Subst_WellTyped funcs U G sub ->
-        forall l1 : list (expr types),
-          Folds.fold_left_2_opt (exprUnify n) l l1 sub = Some sub' ->
-          Folds.all2 (is_well_typed funcs U G) l1 l0 = true ->
-          Folds.all2 (is_well_typed funcs U G) l l0 = true ->
-          Subst_WellTyped funcs U G sub'.
+            Subst_WellTyped funcs U G sub ->
+            Subst_WellTyped funcs U G sub').
     Proof.
-      induction 1; simpl; intros.
-      { destruct l0; destruct l1; simpl in *; auto; try congruence. inversion H0; subst; auto. }
-      { destruct l1; destruct l0; try congruence. simpl in *.
-        repeat match goal with
-                 | [ H : context [ match ?X with 
-                                     | _ => _ 
-                                   end ] |- _ ] =>
-                 revert H; case_eq X; try congruence; intros
-               end. eauto. }
-    Qed.    
+      induction n; simpl in *; try congruence.
+      induction l; simpl in *.
+      { destruct r; simpl in *; intros; try congruence.
+        { consider (equiv_dec t t1); unfold equiv in *; simpl in *; intros; subst; try congruence.
+          consider (get_Eq types t1 t0 t2); try congruence; simpl in *; intros.
+          inversion H0; clear H0; subst. split; [ reflexivity | split; [ reflexivity | ] ].
+          intros. consider (tvar_seqb t1 t); intros; subst; auto. }
+        { eapply unify_uvar; eauto. } }
+      { destruct r; simpl in *; intros; try congruence.
+        { consider (Peano_dec.eq_nat_dec x v); try congruence; subst; intros.
+          inversion H; clear H; subst. intuition. }
+        { eapply unify_uvar; eauto. } }
+      { do 4 intro.
+        assert ((exists u, r = UVar u) \/
+                match Subst_lookup x sub with
+                  | Some l' => exprUnify n l' r sub
+                  | None => Subst_set x r sub
+                end = Some sub').
+        { destruct r; auto. left. eauto. }
+        destruct H0.
+        { destruct H0; subst.
+          consider (EqNat.beq_nat x x0); intros; subst.
+          { inversion H0; clear H0; subst. intuition. }
+          { consider (Subst_lookup x sub); intros.
+            { consider (Subst_lookup x0 sub); intros.
+              { repeat rewrite exprInstantiate_UVar.
+                specialize (IHn _ _ _ _ H2). destruct IHn as [ ? [ ? ? ] ].
+                repeat erewrite Subst_lookup_Extends by eassumption.
+                intuition. 
+                simpl in *; consider (nth_error U x); consider (nth_error U x0); intros.
+                consider (tvar_seqb t t0); consider (tvar_seqb t t1); intros.
+                subst.
+                eapply H5 with (t := t0); eauto using Subst_lookup_WellTyped. }
+              { intuition.
+                { erewrite Subst_set_exprInstantiate with (x := x0) by eassumption.
+                  rewrite exprInstantiate_UVar.
+                  erewrite Subst_lookup_Extends; try eassumption.
+                  reflexivity. eapply Subst_set_Extends; eauto. }
+                { eapply Subst_set_Extends; eauto. }
+                { simpl in *. 
+                  consider (nth_error U x); consider (nth_error U x0); intros.
+                  consider (tvar_seqb t t0); consider (tvar_seqb t t1); intros; subst.
+                  eapply Subst_set_WellTyped; try eassumption.
+                  eapply Subst_lookup_WellTyped; try eassumption. } } }
+            { intuition.
+              { erewrite Subst_set_exprInstantiate with (x := x) by eassumption. 
+                reflexivity. }
+              { eapply Subst_set_Extends; eauto. }
+              { simpl in *. 
+                consider (nth_error U x); consider (nth_error U x0); intros.
+                consider (tvar_seqb t t0); consider (tvar_seqb t t1); intros; subst.
+                eapply Subst_set_WellTyped; try eassumption.
+                simpl. rewrite H2. consider (tvar_seqb t0 t0); auto. } } } } 
+        { clear H. consider (Subst_lookup x sub); intros.
+          { specialize (IHn _ _ _ _ H0); intuition.
+            { rewrite exprInstantiate_UVar. 
+              erewrite Subst_lookup_Extends; try eassumption. }
+            { eapply H4; try eassumption.
+              eapply Subst_lookup_WellTyped; eauto.
+              destruct (nth_error U x); try congruence.
+              consider (tvar_seqb t t0); try congruence. } }
+          { intuition. 
+            { erewrite Subst_set_exprInstantiate by eassumption. auto. }
+            { eapply Subst_set_Extends; eauto. }
+            { eapply Subst_set_WellTyped; eauto.
+              destruct (nth_error U x); try congruence.
+              consider (tvar_seqb t t0); try congruence. } } } }
+      { destruct r; simpl in *; intros; try congruence.
+        { consider (EqNat.beq_nat f f0); try congruence; intros; subst.
+          intros. apply and_assoc. 
+          split.
+          { generalize dependent l0; generalize dependent sub; generalize dependent sub'.
+            induction H.
+            { destruct l0; try congruence. inversion 1; subst. intuition. }
+            { destruct l0; try congruence; intros.
+              match goal with
+                | [ H : match ?X _ _ _ with _ => _ end = _ |- _ ] =>
+                  generalize dependent X; intros
+              end.
+              consider (o x e sub); try congruence; intros.
+              specialize (H _ _ _ H1). specialize (IHForall _ _ _ H2). clear H2.
+              intuition.
+              { simpl. inversion H; clear H; subst.
+                repeat rewrite exprInstantiate_Func in *.
+                simpl. f_equal. f_equal; auto.
+                erewrite <- exprInstantiate_Extends with (y := s); eauto. rewrite H2.
+                rewrite exprInstantiate_Extends; auto. }
+              { etransitivity; eauto. } } }
+          { intros. destruct (nth_error funcs f0); try congruence.
+            destruct t0. simpl in *.
+            generalize dependent l0; generalize dependent sub; generalize dependent sub'; 
+              generalize dependent TDomain.
+            induction H.
+            { destruct l0; try congruence. inversion 1; subst. 
+              destruct (tvar_seqb t TRange); try congruence. auto. }
+            { destruct l0; try congruence. intros.
+              match goal with
+                | [ H : match ?X _ _ _ with _ => _ end = _ |- _ ] =>
+                  generalize dependent X; intros
+              end.
+              consider (o x e sub); intros; try congruence.
+              specialize (H _ _ _ H2).
+              consider (tvar_seqb t TRange); intros; subst. simpl in *.
+              destruct TDomain; try congruence.
+              consider (is_well_typed funcs U G x t).
+              consider (is_well_typed funcs U G e t).
+              intuition. eapply H7. 3: eapply H5. eassumption. eauto. eauto. } } }
+        { eapply unify_uvar; eauto. } }
+      { destruct r; intros; try congruence.
+        { consider (equiv_dec t t0); try congruence; unfold equiv in *; simpl in *; intros; subst.
+          match goal with
+            | [ H : match ?X _ _ _ with _ => _ end = _ |- _ ] =>
+              generalize dependent X; intros
+          end.
+          consider (o l1 r1 sub); try congruence; intros.
+          specialize (IHl1 _ _ _ H). specialize (IHl2 _ _ _ H0).
+          intuition.
+          { do 2 rewrite exprInstantiate_Equal. f_equal; auto. 
+            erewrite <- exprInstantiate_Extends with (y := s); eauto. rewrite H1.
+            rewrite exprInstantiate_Extends; auto. }
+          { etransitivity; eauto. }
+          { destruct t; try congruence.
+            eapply andb_true_iff in H4. eapply andb_true_iff in H8. intuition eauto. } }
+        { eapply unify_uvar; eauto. } }
+      { destruct r; intros; try congruence.
+        { specialize (IHl _ _ _ H). clear H. intuition eauto. 
+          repeat rewrite exprInstantiate_Not. rewrite H. auto.
+          destruct t; try congruence. simpl in *. eauto. } 
+        { eapply unify_uvar; eauto. } }
+    Qed.
+
+    Transparent Subst_set.
+
+    Theorem exprUnify_sound : forall n l r sub sub',
+      exprUnify n l r sub = Some sub' ->
+      exprInstantiate sub' l = exprInstantiate sub' r.
+    Proof.
+      intros. specialize (exprUnify_all _ _ _ _ H); intuition.
+    Qed.
+
+    Theorem exprUnify_sound' : forall n l r sub sub',
+      exprUnify n l r sub = Some sub' ->
+      forall funcs U G t,
+      exprD funcs U G (exprInstantiate sub' l) t = 
+      exprD funcs U G (exprInstantiate sub' r) t.
+    Proof.
+      intros. f_equal. specialize (exprUnify_all _ _ _ _ H); intuition. 
+    Qed.
+
+    Theorem exprUnify_Extends : forall n l r sub sub',
+      exprUnify n l r sub = Some sub' ->
+      Subst_Extends sub' sub.
+    Proof.
+      intros. specialize (exprUnify_all _ _ _ _ H); intuition.
+    Qed.
 
     Theorem exprUnify_WellTyped : forall n l r sub sub',
       exprUnify n l r sub = Some sub' ->
@@ -1451,61 +1261,18 @@ Module SynUnifier (E : OrderedType.OrderedType with Definition t := uvar with De
         Subst_WellTyped funcs U G sub ->
         Subst_WellTyped funcs U G sub'.
     Proof.
-      induction n; induction l; intros; rewrite exprUnify_unroll in *; unfold get_Eq in *; destruct r; simpl in *;
-        try congruence;
-        repeat (match goal with
-                 | [ H : (if ?X then _ else _) = _ |- _ ] =>
-                   (revert H; Reflection.consider X; intros; try congruence); [ try subst ]
-                 | [ H : context [ @equiv_dec ?A ?B ?C ?E ?X ?Y ] |- _ ] =>
-                   destruct (@equiv_dec A B C E X Y); unfold equiv in *; subst; try congruence
-                 | [ H : context [ match ?T with
-                                     | tvProp => _
-                                     | tvType _ => _
-                                   end ] |- _ ] => (destruct T; try congruence); [ ] 
-                 | [ H : context [ match nth_error ?X ?Y with
-                                     | _ => _ 
-                                   end ] |- _ ] => 
-                 revert H; case_eq (nth_error X Y); intros; try congruence
-                 | [ H : context [ match Subst_lookup ?X ?Y with
-                                     | _ => _ 
-                                   end ] |- _ ] => 
-                 revert H; case_eq (Subst_lookup X Y); intros; try congruence
-                 | [ H : (if ?X then _ else _) = _ |- _ ] =>
-                   (revert H; Reflection.consider X; intros; try congruence); [ ]
-                 | [ H : ?X = _ , H' : ?X = _ |- _ ] => rewrite H in H'
-                 | [ H : Some _ = Some _ |- _ ] => inversion H; clear H; subst
-                 | [ H : context [ match exprUnify ?A ?B ?C ?D with _ => _ end ] |- _ ] => 
-                   revert H; case_eq (exprUnify A B C D); intros; try congruence
-                 | [ H : _ && _ = true |- _ ] => eapply andb_true_iff in H; destruct H
-                 | [ H : forall a b c d, exprUnify ?n a b c = Some d -> _ , H' : exprUnify ?n _ _ _ = Some _ |- _ ] =>
-                   (eapply H in H'; (eauto using Subst_lookup_WellTyped, Subst_set_WellTyped with exprs)); 
-                   instantiate; eauto with exprs
-                 | [ H : ?X = ?X , H' : context [ match ?H with _ => _ end ] |- _ ] =>
-                   rewrite (EqdepClass.UIP_refl H) in H'
-                 | [ |- _ ] => try unfold equiv in *; progress subst 
-               end);
-        try solve [ eauto using Subst_lookup_WellTyped, Subst_set_WellTyped with exprs
-              | (eapply Subst_set_WellTyped; eauto); simpl;
-                repeat match goal with
-                         | [ H : _ = _ |- _ ] => rewrite H
-                         | [ |- _ ] => rewrite EquivDec_refl_left
-                         | [ |- _ ] => rewrite tvar_seqb_refl
-                       end; auto 
-          | eauto using exprUnify_WellTyped_Forall].
-      { consider (EqNat.beq_nat x u); intros; subst.
-        inversion H4; clear H4; subst; auto. 
-        eapply Subst_set_WellTyped; try eassumption.
-        simpl. rewrite H1. consider (tvar_seqb t t); auto. }
-      { consider (EqNat.beq_nat x u); intros; subst.
-        inversion H5; clear H5; subst; auto. 
-        eapply IHn. eassumption. 3: eassumption. 
-        eapply Subst_lookup_WellTyped; eassumption.
-        eapply Subst_lookup_WellTyped; eassumption. }
-      { consider (EqNat.beq_nat x u); intros; subst.
-        inversion H4; clear H4; subst; auto. 
-        eapply Subst_set_WellTyped; try eassumption.
-        simpl. rewrite H1. consider (tvar_seqb t t); auto. }
+      do 6 intro. specialize (exprUnify_all _ _ _ _ H); intuition.
     Qed.
+
+    Opaque Subst_lookup.
+
+    Hint Extern 1 (is_well_typed _ _ _ _ _ = _) =>
+      simpl;
+        repeat match goal with 
+                 | [ H : _ = _ |- _ ] => rewrite H
+                 | [ |- _ ] => rewrite EquivDec_refl_left
+                 | [ |- _ ] => rewrite tvar_seqb_refl
+               end; reflexivity : exprs.
 
     Lemma Subst_lookup_Subst_equations : forall funcs U G x sub e t,
       Subst_lookup x sub = Some e ->
@@ -1566,7 +1333,7 @@ Module SynUnifier (E : OrderedType.OrderedType with Definition t := uvar with De
       { change (FM.find x (projT1 sub)) with (Subst_lookup x sub). 
         case_eq (Subst_lookup x sub); intros; simpl; auto.        
         erewrite Subst_lookup_Subst_equations; eauto. }
-      { destruct (nth_error funcs f); auto.
+      { simpl. destruct (nth_error funcs f); auto.
         destruct (equiv_dec (Range s) t); auto. unfold equiv in *. subst.
         destruct s; simpl in *.  
         generalize dependent Domain. induction H; destruct Domain; simpl; auto.
@@ -1601,6 +1368,8 @@ Module SynUnifier (E : OrderedType.OrderedType with Definition t := uvar with De
       revert H1. induction H; think.
     Qed.
 
+    Transparent exprInstantiate.
+
     Theorem exprInstantiate_Removes : forall k sub e e' e'',
       Subst_lookup k sub = Some e ->
       exprInstantiate sub e' = e'' ->
@@ -1610,7 +1379,8 @@ Module SynUnifier (E : OrderedType.OrderedType with Definition t := uvar with De
       { destruct sub. unfold Subst_lookup, subst_lookup in *; simpl in *.
         consider (FM.find x x0); intros; simpl.
         2: consider (EqNat.beq_nat k x); try congruence.
-        eapply normalized_not_mentions. eapply H. eapply w. eapply FACTS.find_mapsto_iff. eauto. }
+        eapply normalized_not_mentions. eapply H. eapply w. eapply FACTS.find_mapsto_iff.
+        eauto. }
       { induction H; simpl; auto. rewrite H; auto. }
     Qed.
 
